Makefile
@@ -2,11 +2,10 @@ include Makefile.include
 
 #FSTAR_HOME=/opt/FStar
 #FSTAR_BIN=fstar.exe
-#FSTAR_MONO=mono
 #TIMEOUT=100
-DEFTIMEOUT=50
+DEFTIMEOUT=5
 
-FSTAR=$(FSTAR_MONO) $(FSTAR_HOME)/bin/$(FSTAR_BIN) --n_cores 1 --max_fuel 1 --max_ifuel 1 --fstar_home $(FSTAR_HOME)
+FSTAR=$(FSTAR_HOME)/bin/$(FSTAR_BIN) --n_cores 1 --max_fuel 1 --max_ifuel 1 --fstar_home $(FSTAR_HOME)
 
 all : stlc-norm
 
